src/Refinement.v
@@ -16,6 +16,22 @@ Proof.
   intros A B H H0. apply H. apply H0.
 Qed.
 
+Definition of_same_length_eq_l {A B} {l1 l1' : list A} {l2 : list B} (H : OfSameLength l1 l2) :
+  l1 = l1' →
+  OfSameLength l1' l2.
+Proof. intros. subst. exact H. Qed.
+
+Definition of_same_length_eq_r {A B} {l1 : list A} {l2 l2' : list B} (H : OfSameLength l1 l2) :
+  l2 = l2' →
+  OfSameLength l1 l2'.
+Proof. intros. subst. exact H. Qed.
+
+Definition of_same_length_eq {A B} {l1 l1' : list A} {l2 l2' : list B} (H : OfSameLength l1 l2) :
+  l1 = l1' →
+  l2 = l2' →
+  OfSameLength l1' l2'.
+Proof. intros. subst. exact H. Qed.
+
 Open Scope stdpp_scope.
 Open Scope refiney_scope.
 
@@ -376,20 +392,49 @@ Section refinement.
     apply f_foralllist_drop_binders.
   Qed.
 
-  Lemma f_eqlist_fmap_app {X} (l1 l2 : list X) (f : X → term) (g : X → term)
-                          `{OfSameLength _ _ (f <$> l1 ++ l2) (g <$> l1 ++ l2)}
-                          `{OfSameLength _ _ (f <$> l1) (g <$> l1)}
-                          `{OfSameLength _ _ (f <$> l2) (g <$> l2)} :
-    <! ⌜$(f <$> l1 ++ l2) =* $(g <$> l1 ++ l2)⌝ !> ≡
-       <! ⌜$(f <$> l1) =* $(g <$> l1)⌝ ∧ ⌜$(f <$> l2) =* $(g <$> l2)⌝ !>.
+  Lemma f_eqlist_app ts1 ts1' ts2 ts2'
+                          `{OfSameLength _ _ (ts1 ++ ts1') (ts2 ++ ts2')}
+                          `{OfSameLength _ _ ts1 ts2}
+                          `{OfSameLength _ _ ts1' ts2'} :
+    <! ⌜$(ts1 ++ ts1') =* $(ts2 ++ ts2')⌝ !> ≡@{formula}
+       <! ⌜$(ts1) =* $(ts2)⌝ ∧ ⌜$(ts1') =* $(ts2')⌝ !>.
   Proof with auto.
-    induction l1 as [|x l1 IH]; simpl.
-    - rewrite f_eqlist_nil. f_simpl. f_equiv. apply eq_pi. solve_decision.
-    - do 2 rewrite f_eqlist_cons. rewrite <- f_and_assoc. f_simpl.
-      rewrite IH...
-      Unshelve.
-      all: typeclasses eauto.
+    generalize dependent ts2.
+    induction ts1 as [|t1 ts1 IH]; simpl; intros; assert (Hl:=H0).
+    - apply of_same_length_nil_inv_l in Hl as ->. simpl. rewrite f_eqlist_nil.
+      f_simpl. f_equiv. apply OfSameLength_pi.
+    - apply of_same_length_cons_inv_l in Hl as (t2&ts2''&->&?). rename ts2'' into ts2.
+      simpl. repeat rewrite f_eqlist_cons. rewrite <- f_and_assoc. f_simpl.
+      rewrite IH... Unshelve.
+      + simpl in H. apply of_same_length_rest in H...
+      + apply of_same_length_rest in H0...
   Qed.
+
+  Lemma f_eqlist_replace_l ts1 ts1' ts2 {H : OfSameLength ts1 ts2} (Heq : ts1 = ts1') :
+    @FEqList _ ts1 ts2 H ≡@{formula} @FEqList _ ts1' ts2 (of_same_length_eq_l H Heq).
+  Proof. subst. f_equiv. apply OfSameLength_pi. Qed.
+
+  Lemma f_eqlist_replace_r ts1 ts2 ts2' {H : OfSameLength ts1 ts2} (Heq : ts2 = ts2') :
+    @FEqList _ ts1 ts2 H ≡@{formula} @FEqList _ ts1 ts2' (of_same_length_eq_r H Heq).
+  Proof. subst. f_equiv. apply OfSameLength_pi. Qed.
+
+  Lemma f_eqlist_replace {ts1 ts1' ts2 ts2'} {H : OfSameLength ts1 ts2} :
+    ∀ Heq1 : ts1 = ts1',
+    ∀ Heq2 : ts2 = ts2',
+    @FEqList _ ts1 ts2 H ≡@{formula} @FEqList _ ts1' ts2' (of_same_length_eq H Heq1 Heq2).
+  Proof. intros. subst. f_equiv. apply OfSameLength_pi. Qed.
+
+(* Ltac split_eqlist_fmap_app l1 l2 f g := *)
+(*   repeat match goal with *)
+(*     | H : context[@FEqList (f <$> l1 ++ l2) (f <$> l1 ++ l2) ?Hlength] |- _ => *)
+(*         rewrite (@f_eqlist_fmap_app _ l1 l2 ?f ?g ?Hlength _ _) in H *)
+(*     | |- context[@FEqList (f <$> l1 ++ l2) (g <$> l1 ++ l2) ?Hlength] => *)
+(*         assert (True); *)
+(*         rewrite (@f_eqlist_fmap_app _ l1 l2 ?f ?g ?Hlength _ _) *)
+(*     | |- context[FEqList (?f <$> ?l1) ?l2] => *)
+(*         let H := fresh in *)
+(*         idtac f l1 *)
+(*     end. *)
 
 
 Notation "' xs" := (TVar ∘ as_var <$> xs : list term)
@@ -398,6 +443,60 @@ Notation "' xs" := (TVar ∘ as_var <$> xs : list term)
 Notation "'₀ xs" := (TVar ∘ initial_var_of <$> xs : list term)
                        (in custom term at level 0,
                            xs constr at level 0) : refiney_scope.
+  Lemma subst_initials_seqsubst_lists_unique xs :
+    @seqsubst_lists_unique M (initial_var_of <$> xs) (TVar ∘ as_var <$> xs).
+  Proof.
+    unfold seqsubst_lists_unique. intros.
+    rewrite elem_of_list_pair_indexed in H0, H1. destruct H0 as []. destruct H1 as [].
+    apply list_lookup_fmap_inv in H0 as (x1&?&?).
+    apply list_lookup_fmap_inv in H1 as (x2&?&?).
+    apply list_lookup_fmap_inv in H2 as (x3&?&?).
+    apply list_lookup_fmap_inv in H3 as (x4&?&?).
+    rewrite H4 in H6. inversion H6. subst x3. rewrite H5 in H7.
+    inversion H7. subst x4. clear H6 H7. rewrite H0 in H1.
+    rewrite H2. rewrite H3. f_equal. apply initial_var_of_inj in H1. assumption.
+  Qed.
+
+  Lemma subst_initials_vars_terms_disjoin xs :
+    list_to_set (initial_var_of <$> xs) ## ⋃ (@term_fvars value <$> (TVar ∘ as_var <$> xs)).
+  Proof.
+    (* Set Printing Coercions. Unset Printing Notations. *)
+    intros x0 H1 H2. set_unfold. destruct H1 as (x&?&?). subst.
+    apply elem_of_union_list in H2 as (fvars&?&?).
+    apply elem_of_list_fmap in H as (x1&?&?). apply elem_of_list_fmap in H2 as (x2&?&?).
+    subst x1. simpl in H. subst fvars. apply elem_of_singleton in H1.
+    apply initial_var_of_eq_final_variable in H1 as [].
+  Qed.
+
+  Hint Resolve subst_initials_seqsubst_lists_unique : core.
+  Hint Resolve subst_initials_vars_terms_disjoin : core.
+
+  Lemma fold_subst_initials A w :
+    seqsubst A (initial_var_of <$> w) (TVar ∘ as_var <$> w) = <! A[_₀\ w] !>.
+  Proof. reflexivity. Qed.
+
+  Lemma seqsubst_non_free A (xs : list variable) ts `{OfSameLength _ _ xs ts} :
+    formula_fvars A ## list_to_set xs →
+    <! A[; *xs \ *ts ;] !> ≡ A.
+  Proof with auto.
+    generalize dependent ts. induction xs as [|x xs IH]; intros; assert (Hl:=H).
+    - apply of_same_length_nil_inv_l in Hl as ->. simpl...
+    - apply of_same_length_cons_inv_l in Hl as (t&ts'&->&?). rename ts' into ts. simpl...
+      rewrite IH.
+      2:{ set_solver. }
+      rewrite fequiv_subst_non_free... set_solver.
+  Qed.
+
+  Lemma f_drop_subst_initials A w :
+    formula_final A →
+    <! A[_₀\ w] !> ≡ A.
+  Proof.
+    intros. unfold subst_initials. apply seqsubst_non_free. intros x0 ? ?.
+    set_unfold. destruct H1 as (x&?&?). apply H in H0. unfold var_final in H0.
+    rewrite H1 in H0. simpl in H0. discriminate.
+  Qed.
+
+
   Lemma r_assignment w xs pre post ts `{FormulaFinal _ pre} `{OfSameLength _ _ xs ts} :
     length xs ≠ 0 →
     NoDup xs →
@@ -405,36 +504,63 @@ Notation "'₀ xs" := (TVar ∘ initial_var_of <$> xs : list term)
     <{ *w, *xs : [pre, post] }> ⊑ <{ *xs := *$(FinalRhsTerm <$> ts)  }>.
   Proof with auto.
     intros Hlength Hnodup proviso A Hfinal. simpl. rewrite wp_asgn.
-    assert (<! pre !> ≡ <! pre [_₀\w ++ xs] !>).
-    { admit. }
-    rewrite H1. clear H1. rewrite <- simpl_subst_initials_and. rewrite fmap_app.
-    unfold subst_initials.
-    rewrite <- f_foralllist_one_point.
-    2:{ unfold seqsubst_lists_unique. intros.
-        rewrite elem_of_list_pair_indexed in H2, H3. destruct H2 as [].
-        destruct H3.
-        apply list_lookup_fmap_inv in H2 as (x1&?&?).
-        apply list_lookup_fmap_inv in H3 as (x2&?&?).
-        apply list_lookup_fmap_inv in H4 as (x3&?&?).
-        apply list_lookup_fmap_inv in H5 as (x4&?&?).
-        rewrite H6 in H8. inversion H8. subst x3. rewrite H7 in H9.
-        inversion H9. subst x4. clear H8 H9. rewrite H2 in H3.
-        rewrite H4. rewrite H5. f_equal. apply initial_var_of_inj in H3... }
-    2: { set_unfold. intros x0. intros ((x&?&?)&?).
-         apply elem_of_union_list in H3 as (fvars&?&?).
-         apply elem_of_list_fmap in H3 as (x1&?&?).
-         apply elem_of_list_fmap in H5 as (x2&?&?). subst x1. simpl in H3.
-         subst fvars. apply elem_of_singleton in H4. subst x0.
-         apply initial_var_of_ne in H4 as []. }
+    assert (<! pre !> ≡ <! pre [_₀\w ++ xs] !>) as ->.
+    { rewrite f_drop_subst_initials... }
+    rewrite <- simpl_subst_initials_and. rewrite fmap_app.
+    unfold subst_initials. rewrite <- f_foralllist_one_point...
     rewrite f_foralllist_app. rewrite (f_foralllist_drop_binders (as_var <$> w)).
     rewrite (f_foralllist_elim_as_ssubst <! post ⇒ A !> _ (as_term <$> ts))...
     2:{ rewrite length_fmap... }
     2:{ apply NoDup_fmap... apply as_var_inj. }
+    erewrite f_eqlist_replace. Unshelve.
+    4: { do 2 rewrite fmap_app. do 2 rewrite <- list_fmap_compose. reflexivity. }
+    3: { rewrite fmap_app. reflexivity. }
+    rewrite f_eqlist_app. rewrite f_impl_dup_hyp. rewrite (f_and_assoc _ pre).
+    rewrite f_and_assoc in proviso. rewrite proviso. clear proviso. rewrite simpl_ssubst_impl.
+    f_simpl. rewrite <- f_eqlist_app.
+    erewrite f_eqlist_replace. Unshelve.
+    5: { rewrite <- fmap_app. rewrite list_fmap_compose. reflexivity. }
+    3: { rewrite <- fmap_app. reflexivity. }
+    pose proof (@f_foralllist_one_point M
+                  (initial_var_of <$> (w ++ xs)) ((TVar ∘ as_var <$> (w++xs)))) as ->...
+    rewrite fold_subst_initials. rewrite f_drop_subst_initials.
+    2: { unfold formula_final. intros. apply fvars_ssubst_superset in H1.
+         set_unfold. destruct H1.
+         - apply Hfinal...
+         - apply elem_of_union_list in H1 as (fvars&?&?).
+           apply elem_of_list_fmap in H1 as (t&->&?).
+           apply elem_of_list_fmap in H1 as (t'&->&?).
+           pose proof (final_term_final t').
+           apply H3... }
+    reflexivity.
+  Qed.
+
+    rewrite H1... rewrite simult_subst_
+    2: {  }
+
+    Set Printing Coercions.
+    rewrite f_foralllist_one_point.
+    4: { do 2 rewrite fmap_app. do 2 rewrite <- list_fmap_compose. reflexivity. }
+    3: { rewrite fmap_app. reflexivity. }
+    2:{ rewrite length_fmap... }
+    2:{ apply NoDup_fmap... apply as_var_inj. }
+    erewrite f_eqlist_replace. Unshelve.
+    rewrite f_foralllist_impl_unused_r.
+    rewrite f_impl_elim.
+    f_impl_elim
+    rewrite <- f_and_assoc at 2.
+    rewrite proviso.
+    Unshelve.
+    pose proof (fmap_app ((@TVar value) ∘ as_var) w xs).
+    assert (OfSameLength (initial_var_of <$> w ++ xs) ((@TVar value) ∘ as_var <$> w ++ xs) =
+ OfSameLength (initial_var_of <$> w ++ xs) ((TVar ∘ as_var <$> w) ++ ((@TVar value) ∘ as_var <$> xs))).
+    { rewrite H1. reflexivity. }
+    Unset Printing Notations. Set Printing Implicit.
     rewrite simpl_ssubst_impl.
-    setoid_rewrite fmap_app.
+    split_eqlist_fmap_app w xs (initial_var_of) ((@TVar (value)) ∘ as_var).
+
     clear.
     pose proof (f_eqlist_fmap_app w xs (initial_var_of) (TVar ∘ as_var)).
-    Unset Printing Notations. Set Printing Implicit.
     unfold fmap.
     rewrite H1.
 
